SPF_JB.thy
@@ -743,11 +743,11 @@ lemma spfapply_in_out:
   
 
 subsection \<open>spfRt lemma\<close>
-lemma spfrt_step: "(spfRt\<cdot>spf)\<rightleftharpoons>sb = spf\<rightleftharpoons>(sbRt\<cdot>sb)"
+lemma spfrt_step[simp]: "(spfRt\<cdot>spf)\<rightleftharpoons>sb = spf\<rightleftharpoons>(sbRt\<cdot>sb)"
   by(simp add: spfRt_def)
 
 subsection \<open>spfConc lemma\<close>
-lemma spconc_step: 
+lemma spconc_step[simp]: 
   shows "(spfConc sb1\<cdot>spf)\<rightleftharpoons>sb2 = sbConc sb1\<cdot>(spf\<rightleftharpoons>sb)"
   apply(simp add: spfConc_def)
   sorry
